move ifthenelse rule from examples into ifc

examples/write_labeled_val_verif.v
@@ -1,3 +1,4 @@
+Require Import ifc.rules.
 Require Import ifc.ifc.
 Require Import floyd.proofauto.
 Require Import examples.write_labeled_val.
@@ -13,23 +14,6 @@ Instance Espec: OracleKind. Admitted.
 
 Axiom ifc_core0_always_holds: forall {T: Type} Delta P N A c P' N' A',
   @ifc_core T Delta P N A c P' N' A'.
-
-(* We need lifting on top of VST's lifting... *)
-
-Definition iand{A: Type}(P1: A -> pre_assert)(P2: A -> pre_assert): A -> pre_assert :=
-  fun (x: A) => (P1 x) && (P2 x).
-
-Definition iprop{A: Type}(P: pre_assert): A -> pre_assert := fun (_: A) => P.
-
-Lemma ifc_ifthenelse: forall {T: Type} {cs: compspecs} {Espec: OracleKind} (Delta: tycontext) 
-  (P: T -> pre_assert) (N: T -> stack_clsf) (A: T -> heap_clsf)
-  (b: expr) (c1 c2: statement)
-  (P': T -> ret_assert) (N': T -> stack_clsf) (A': T -> heap_clsf),
-  bool_type (typeof b) = true ->
-  ifc_def Delta (iand P (iprop (local (`(typed_true  (typeof b)) (eval_expr b))))) N A c1 P' N' A' ->
-  ifc_def Delta (iand P (iprop (local (`(typed_false (typeof b)) (eval_expr b))))) N A c2 P' N' A' ->
-  ifc_def Delta P N A (Sifthenelse b c1 c2) P' N' A'.
-Admitted.
 
 (* alternative: give an explicit constructor name
 Record MyMetaVars: Type := mkMyMetaVars { v: int; b: int; highptr: val; lowptr: val }.
