ifc/rules.v
@@ -1,0 +1,34 @@
+Require Import compcert.cfrontend.Clight.
+Require Import veric.Clight_new.
+Require Import compcert.lib.Maps. (* for PMap and ZMap *)
+Require Import compcert.lib.Integers.
+Require Import compcert.common.Values.
+Require Import compcert.common.Memory.
+Require Import floyd.base.
+Require Import ifc.ifc.
+Require Import lib.LibTactics.
+
+Local Open Scope logic.
+
+(* We need lifting on top of VST's lifting... *)
+
+Definition iand{A: Type}(P1: A -> pre_assert)(P2: A -> pre_assert): A -> pre_assert :=
+  fun (x: A) => (P1 x) && (P2 x).
+
+Definition iprop{A: Type}(P: pre_assert): A -> pre_assert := fun (_: A) => P.
+
+Section RULES.
+Context (Espec : OracleKind).
+Context (CS: compspecs).
+
+Lemma ifc_ifthenelse: forall {T: Type} (Delta: tycontext) 
+  (P: T -> pre_assert) (N: T -> stack_clsf) (A: T -> heap_clsf)
+  (b: expr) (c1 c2: statement)
+  (P': T -> ret_assert) (N': T -> stack_clsf) (A': T -> heap_clsf),
+  bool_type (typeof b) = true ->
+  ifc_def Delta (iand P (iprop (local (`(typed_true  (typeof b)) (eval_expr b))))) N A c1 P' N' A' ->
+  ifc_def Delta (iand P (iprop (local (`(typed_false (typeof b)) (eval_expr b))))) N A c2 P' N' A' ->
+  ifc_def Delta P N A (Sifthenelse b c1 c2) P' N' A'.
+Admitted.
+
+End RULES.
